

1. EXPANSION OF THE 3RD ORDER 3-STEP SSPX METHOD (SPECIAL FORM)

We are solving numerically the equation

$$u' = F(u).$$

Let t_0 be the initial time, and correspondingly $u_0 = u(t_0)$. Expanding the exact solution gives

$$(1.1) \quad \begin{aligned} u(t_0 + \Delta t) = & u_0 + \Delta t F(u_0) + \frac{(\Delta t)^2}{2} F'(u_0) F(u_0) \\ & + \frac{(\Delta t)^3}{6} [F''(u_0)(F(u_0))^2 + (F'(u_0))^2 F(u_0)] + o((\Delta t)^3). \end{aligned}$$

The special method takes the form

$$\begin{aligned} u_1 &= u_0 + a_1 \Delta t F(u_0), \\ \tilde{u} &= (1 - w_1) u_0 + w_1 u_1, \\ u_2 &= \tilde{u} + a_2 \Delta t F(u_1), \\ \bar{u} &= (1 - w_2) u_0 + w_2 u_2, \\ u_3 &= \bar{u} + a_3 \Delta t F(u_2). \end{aligned}$$

We now expand the numerical scheme:

$$\begin{aligned} \tilde{u} &= u_0 + w_1 a_1 \Delta t F(u_0), \\ u_2 &= u_0 + w_1 a_1 \Delta t F(u_0) + a_2 \Delta t F(u_0 + a_1 \Delta t F(u_0)) \\ &= u_0 + \underbrace{w_1 a_1 \Delta t F(u_0) + a_2 \Delta t (F(u_0) + a_1 \Delta t F(u_0) F'(u_0) + 2^{-1} (a_1 \Delta t F(u_0))^2 F''(u_0))}_{:=h} + o((\Delta t)^3). \end{aligned}$$

Remark 1.1. The o symbol implicitly has dependence on $F(u_0)$ and its derivatives, which means the approximation could be bad if F and its derivatives are very big.

So that

$$(1.2) \quad h = (w_1 a_1 + a_2) \Delta t F(u_0) + a_1 a_2 (\Delta t)^2 F(u_0) F'(u_0) + 2^{-1} a_1^2 a_2 (\Delta t)^3 (F(u_0))^2 F''(u_0)$$

Then,

$$\bar{u} = u_0 + w_2 h + o((\Delta t)^3).$$

Finally,

$$\begin{aligned} u_3 &= u_0 + w_2 h + a_3 \Delta t F(u_0 + h) + o((\Delta t)^3) \\ &= u_0 + w_2 h + a_3 \Delta t (F(u_0) + h F'(u_0) + 2^{-1} h^2 F''(u_0)) + o((\Delta t)^3) \\ &= u_0 + w_2 \{ (w_1 a_1 + a_2) \Delta t F(u_0) + a_1 a_2 (\Delta t)^2 F(u_0) F'(u_0) + 2^{-1} a_1^2 a_2 (\Delta t)^3 (F(u_0))^2 F''(u_0) \} \\ &\quad + a_3 \Delta t \{ F(u_0) + ((w_1 a_1 + a_2) \Delta t F(u_0) + a_1 a_2 (\Delta t)^2 F(u_0) F'(u_0)) F'(u_0) \\ &\quad + 2^{-1} (w_1 a_1 + a_2)^2 (\Delta t)^2 (F(u_0))^2 F''(u_0) \} + o((\Delta t)^3). \end{aligned}$$

Comparing with expression 1.1, we obtain the following conditions in order for the method to be 3rd order:

$$(1.3) \quad w_2(w_1 a_1 + a_2) + a_3 = 1 \quad (F(u_0) \Delta t),$$

$$(1.4) \quad w_2 a_1 a_2 + a_3(w_1 a_1 + a_2) = \frac{1}{2} \quad (F'(u_0) (\Delta t)^2),$$

$$(1.5) \quad a_1 a_2 a_3 = \frac{1}{6} \quad (F(u_0) (F'(u_0))^2 (\Delta t)^3),$$

$$(1.6) \quad \frac{1}{2} w_2 a_1^2 a_2 + a_3 \frac{1}{2} (w_1 a_1 + a_2)^2 = \frac{1}{6} \quad ((F(u_0))^2 F''(u_0) (\Delta t)^3).$$

Let us set $B := w_1 a_1 + a_2$. The system then yields

$$(1.7) \quad w_2 B + a_3 = 1,$$

$$(1.8) \quad w_2 + 6a_3^2 B = 3a_3,$$

$$(1.9) \quad a_1 a_2 a_3 = \frac{1}{6},$$

$$(1.10) \quad w_2 a_1 + 6a_3^2 B^2 = 2a_3.$$

Then $B = (1 - a_3)/w_2$. Substituting in 1.8 and 1.9 we have:

$$\begin{aligned} w_2^2 + 6a_3^2(1 - a_3) &= 3a_3 w_2, \\ w_2^3 a_1 + 6a_3^2(1 - a_3)^2 &= 2a_3 w_2^2. \end{aligned}$$

From the first we solve for w_2 :

$$w_2 = \frac{3a_3 \pm \sqrt{9a_3^2 - 24a_3^2(1 - a_3)}}{2}.$$

In order for w_2 to be a real number, we need $a_3 \geq 5/8$. We also want $a_3 \leq 1$, otherwise the method has no gain.

We obtain

$$a_1 = \frac{2a_3(w_2(a_3))^2 - 6a_3^2(1 - a_3)^2}{(w_2(a_3))^3}$$

Let's first focus on the $-$ sign in w_2 . From $5/8$ to 1 , w_2 is a decreasing function of a_3 . a_1 , instead, is increasing in a_3 . $a_1(5/8) = 14/15$, and $a_1(2/3) = 1$. So $\max(a_1, a_2, a_3) \geq 1$ if $a_3 \geq 2/3$, hence it suffices to focus on the interval $a_3 \in [5/8, 2/3) = I$. Clearly, on I , $\max(a_1(a_3), a_3) = a_1(a_3)$, as $2/3 < 14/15$. Also, since $a_1 a_2 a_3 = \frac{1}{6}$, on I

$$\frac{5}{8} \frac{14}{15} a_2 \leq \frac{1}{6} \implies a_2 \leq \frac{2}{7} \implies \max(a_1, a_2, a_3) = a_1.$$

This means that the optimum is achieved for $a_3 = \frac{5}{8}$, $a_1 = \frac{14}{15}$, $a_2 = \frac{2}{7}$. We find w_1 from 1.3:

$$w_2(w_1 a_1 + a_2) + a_3 = 1 \implies w_1 = a_1^{-1}(w_2^{-1}(1 - a_3) - a_2) = \frac{15}{14} \left(\frac{16}{15} \frac{3}{8} - \frac{2}{7} \right) = \frac{6}{49}.$$

Then, $\min a_{\max} = \frac{14}{15}$, which means $\Delta t_{\max} \leq \frac{15}{14} \Delta t$. The gain is very small $\sim 7\%$.

Let's now focus on the $+$ case. We have that w_2 is an increasing function of a_3 , and letting

$$A := \frac{1}{3} \left\{ 1 + \frac{(4 + 3\sqrt{2})^{1/3}}{2^{2/3}} - \frac{1}{(2(4 + 3\sqrt{2}))^{1/3}} \right\} \approx 0.6265,$$

we have that $w_2(A) = 1$. We need only to focus on the interval $a_3 \in [5/8, A] = J$. There, a_1 as a function of a_3 is decreasing, and it is such that $a_3(5/8) = \frac{14}{15}$. Also, since $A < \frac{14}{15}$, we will have that $\max(a_1(a_3), a_3) = a_1(a_3)$ on the interval J . By the same reasoning as the previous case, $\max(a_1, a_2, a_3) = a_1$ on J . Hence one just needs to optimize a_1 , and as it is a decreasing function for a_3 , the optimum is achieved for the following choice of parameters:

$$\begin{aligned} a_1 &= a_1(A) \approx 0.9245, \\ a_2 &= \frac{1}{6}(a_1 a_3)^{-1} \approx 0.2877, \\ a_3 &= A \approx 0.6265, \\ w_1 &= a_1^{-1}(w_2^{-1}(1 - a_3) - a_2) \approx 0.0927, \\ w_2 &= 1. \end{aligned}$$

The gain is $\Delta t_{\max} \leq (a_{\max})^{-1} \Delta t \sim (0.9245)^{-1} \Delta t \sim 1.082 \Delta t$.

2. EXPANSION FOR THE SECOND ANSATZ FOR THE METHOD: PARTICULAR CASE $a_1 = a_3$

The second ansatz for the method takes the form

$$(2.1) \quad u_1 = u_0 + a_1 \Delta t F(u_0),$$

$$(2.2) \quad \tilde{u} = (1 - w_1)u_0 + w_1 u_1,$$

$$(2.3) \quad u_2 = \tilde{u} + a_2 \Delta t F(u_1),$$

$$(2.4) \quad \bar{u} = (1 - w_2)\tilde{u} + w_2 u_2,$$

$$(2.5) \quad u_3 = \bar{u} + a_3 \Delta t F(u_2).$$

The calculations go through as in the previous case, with h as before, in 1.2. We have that, in this case,

$$\bar{u} = (1 - w_2)(u_0 + a_1 w_1 \Delta t F(u_0)) + w_2 u_0 + w_2 h = u_0 + a_1 w_1 \Delta t F(u_0) - a_1 w_1 w_2 \Delta t F(u_0) + w_2 h.$$

Since \bar{u} only enters in the first term in Equation 2.5, we obtain the following system:

$$(2.6) \quad w_1 a_1 + w_2 a_2 + a_3 = 1 \quad (F(u_0) \Delta t),$$

$$(2.7) \quad w_2 a_1 a_2 + a_3 (w_1 a_1 + a_2) = \frac{1}{2} \quad (F'(u_0) (\Delta t)^2),$$

$$(2.8) \quad a_1 a_2 a_3 = \frac{1}{6} \quad (F(u_0) (F'(u_0))^2 (\Delta t)^3),$$

$$(2.9) \quad \frac{1}{2} w_2 a_1^2 a_2 + a_3 \frac{1}{2} (w_1 a_1 + a_2)^2 = \frac{1}{6} \quad ((F(u_0))^2 F''(u_0) (\Delta t)^3).$$

Let us make the assumption $a_1 = a_3 := a$. We then obtain the system

$$\begin{aligned} w_1 a + w_2 a_2 + a &= 1, \\ a(w_2 a_2 + w_1 a + a_2) &= \frac{1}{2}, \\ a^2 a_2 &= \frac{1}{6}, \\ \frac{1}{2} w_2 a^2 a_2 + a \frac{1}{2} (w_1 a + a_2)^2 &= \frac{1}{6}. \end{aligned}$$

Upon requiring $a \neq 0$, this is equivalent to

$$(2.10) \quad w_1 a + w_2 a_2 + a = 1,$$

$$(2.11) \quad a(1 - a + a_2) = \frac{1}{2},$$

$$(2.12) \quad a^2 a_2 = \frac{1}{6},$$

$$(2.13) \quad \frac{1}{2} w_2 a^2 a_2 + a \frac{1}{2} (w_1 a + a_2)^2 = \frac{1}{6}.$$

From the first three equations we have that a needs to satisfy the equation of degree 3:

$$a^2 - a^3 + a^2 a_2 = a/2 \implies a^2 - a^3 + 1/6 = a/2 \implies a^3 - a^2 + a/2 - 1/6 = 0.$$

The only positive real solution of this equation is (according to Mathematica):

$$A = \frac{1}{3} \left\{ 1 + \frac{(4 + 3\sqrt{2})^{1/3}}{2^{2/3}} - \frac{1}{(2(4 + 3\sqrt{2}))^{1/3}} \right\} \approx 0.6265,$$

(it is a number that already showed up before). From here, we obtain $a_2 = \frac{a^{-2}}{6} \approx 0.4246$. Substituting $w_2 a_2$ from 2.10 into 2.13, we obtain an equation for w_1 , which is

$$\frac{1}{2} A^2 (1 - A - w_1 A) + \frac{A}{2} (w_1 A + a_2)^2 = \frac{1}{6}.$$

Solving the resulting quadratic equation for w_1 we obtain a unique $w_1 \in [0, 1]$, $w_1 \approx 0.3982$. Plugging those parameters back into Equation 2.10, we obtain a value for $w_2 \approx 0.3735$.

Now, $A^{-1} \approx 1.596$, which is bigger than $\sqrt{2}$.

In this case, A turns out to be **the optimum**, by using Lagrange multipliers (I have a messy Mathematica file with the computations, if needed I can tidy it up).

3. EXPANSION FOR THE THIRD ANSATZ FOR THE METHOD, WITH 6 PARAMETERS

In this case, the method becomes

$$(3.1) \quad u_1 = u_0 + a_1 \Delta t F(u_0),$$

$$(3.2) \quad \tilde{u} = (1 - w_1)u_0 + w_1 u_1,$$

$$(3.3) \quad u_2 = \tilde{u} + a_2 \Delta t F(u_1),$$

$$(3.4) \quad \bar{u} = (1 - w_2 - w_3)u_0 + w_2 u_2 + w_3 u_1,$$

$$(3.5) \quad u_3 = \bar{u} + a_3 \Delta t F(u_2).$$

Calculating the relevant system, it becomes

$$(3.6) \quad w_2(w_1 a_1 + a_2) + w_3 a_1 + a_3 = 1 \quad (F(u_0) \Delta t),$$

$$(3.7) \quad w_2 a_1 a_2 + a_3(w_1 a_1 + a_2) = \frac{1}{2} \quad (F'(u_0)(\Delta t)^2),$$

$$(3.8) \quad a_1 a_2 a_3 = \frac{1}{6} \quad (F(u_0)(F'(u_0))^2(\Delta t)^3),$$

$$(3.9) \quad \frac{1}{2} w_2 a_1^2 a_2 + a_3 \frac{1}{2} (w_1 a_1 + a_2)^2 = \frac{1}{6} \quad ((F(u_0))^2 F''(u_0)(\Delta t)^3).$$

The constraint 3.8 implies that at least one of $\{a_1, a_2, a_3\}$ be greater or equal to $(a_1 a_2 a_3)^{1/3}$. Indeed, if all $a_i < (a_1 a_2 a_3)^{1/3}$, $i = 1, 2, 3$, then multiplying these inequalities together we would get $a_1 a_2 a_3 < a_1 a_2 a_3$, a contradiction. Hence

$$(3.10) \quad \max\{a_1, a_2, a_3\} \geq (a_1 a_2 a_3)^{\frac{1}{3}} \implies \max\{a_1, a_2, a_3\} \geq (1/6)^{\frac{1}{3}}.$$

Hence $a_{\max} \geq (1/6)^{\frac{1}{3}}$.

Let's now set $a_1 = a_2 = a_3$ in addition to the constraints 3.6 – 3.9. This will give 6 equations for 6 unknowns. Hence we solve the system:

$$w_2(w_1 a_1 + a_2) + w_3 a_1 + a_3 = 1,$$

$$w_2 a_1 a_2 + a_3(w_1 a_1 + a_2) = \frac{1}{2},$$

$$a_1 a_2 a_3 = \frac{1}{6},$$

$$\frac{1}{2} w_2 a_1^2 a_2 + a_3 \frac{1}{2} (w_1 a_1 + a_2)^2 = \frac{1}{6},$$

$$a_1 = a_2,$$

$$a_1 = a_3.$$

There is exactly one real solution to this system such that $0 < w_1, w_2, w_3 < 1$. Namely:

$$\begin{aligned}
a_1 &= a_2 = a_3 = (1/6)^{1/3} \approx 0.5503, \\
w_1 &= \frac{1}{2} \left(-1 + \sqrt{9 - 2 \cdot 6^{2/3}} \right) \approx 0.2739, \\
w_2 &= \frac{1}{2} \left(-1 + 6^{2/3} - \sqrt{9 - 2 \cdot 6^{2/3}} \right) \approx 0.3769, \\
w_3 &= \frac{1}{2} \left(2 \cdot 6^{1/3} - 6^{1/3} \right) \approx 0.1661.
\end{aligned}$$

Hence this is the optimum in this case, and the improvement is $a_{\max}^{-1} \approx 1.817$.

4. CAN ANY RUNGE-KUTTA METHOD BE WRITTEN AS COMBINATION OF MIDPOINT STEPS?

I assume here that “combination of s generalized midpoint steps” means a method of the form

$$\begin{aligned}
y_{j+1} &= \bar{y}_j + \alpha_{j+1} \Delta t F(y_j), \quad j = 0, \dots, s, \\
\bar{y}_{j+1} &= \sum_{k=0}^{j+1} \beta_{jk} y_k, \quad j = 0, \dots, s-1.
\end{aligned} \tag{4.1}$$

with the starting values $\bar{y}_0 = y_0 = y(t_n)$, and we let $y(t_{n+1}) := y_s$.

By an s -stage Runge-Kutta method, we denote a method such that

$$\begin{aligned}
k_{i+1} &= F \left(x_0 + \Delta t \sum_{j=1}^i a_{i+1,j} k_j \right), \quad i = 0, \dots, s-1 \\
x(t_{n+1}) &= x_0 + \Delta t \sum_{j=1}^s b_j k_j.
\end{aligned} \tag{4.2}$$

Here, similarly, $x_0 := x(t_n)$.

Let us first remark that an s -stage Runge-Kutta method has $s + s(s-1)/2$ free parameters, whereas a combination of s generalized midpoint steps has $s + s(s+1)/2 - 1$ free parameters.

Proposition 4.1. *An s -stage Runge-Kutta method (as in (4.2)) such that $a_{j+1,j} \neq 0$ for all $j = 1, \dots, s$ can be written as a particular combination of s generalized midpoint steps, as in (4.1).*

Remark 4.2. Notice that the coefficients β in this proposition need not lie in the interval $[0, 1]$. If we were to require this, it would result in a condition on the coefficients a .

Proof. In the definition of Runge-Kutta method, we make the following assumption about notation.

We let, for every $j = 1, \dots, s$,

$$a_{s+1,j} := b_j,$$

so that the method becomes,

$$\begin{aligned}
k_{i+1} &= F \left(x_0 + \Delta t \sum_{j=1}^i a_{i+1,j} k_j \right), \quad i = 0, \dots, s-1 \\
x(t_{n+1}) &= x_0 + \Delta t \sum_{j=1}^s a_{s+1,j} k_j.
\end{aligned} \tag{4.3}$$

Let us now suppose throughout the rest of the proof that $a_{j+1,j} \neq 0$ for all $j = 1, \dots, s$.

We now set up an induction argument.

We denote by $\text{IND}(j)$ the following hypothesis. $\text{IND}(j-1)$ holds if and only if

$$y_k = x_0 + \Delta t \left(\sum_{i=1}^k a_{1+k,i} k_i \right) \tag{4.4}$$

holds for $k = 1, \dots, j-1$, $j \leq s$.

We now check that IND(1) holds trivially. In fact, it is equivalent to

$$y_0 = x_0.$$

We now check that, supposing IND($j-1$), it is possible to deduce IND(j) for some choice of α_j and of $\{\beta_{j-2,q}\}_{q \in \{0, \dots, j-1\}}$. In this step, we assume that the coefficient $\alpha_1, \dots, \alpha_{j-1}$ as well as $\{\beta_{l,p}, (l,p) \text{ such that } l \in \{0, \dots, j-3\}, p \in \{0, \dots, l+1\}\}$ have already been chosen.

Now,

$$y_j = \bar{y}_{j-1} + \alpha_j \Delta t F(y_{j-1}) = \sum_{q=0}^{j-1} \beta_{j-2,q} y_q + \alpha_j \Delta t F(y_{j-1}).$$

By the induction hypothesis,

$$\begin{aligned} \sum_{q=0}^{j-1} \beta_{j-2,q} y_q &= \sum_{q=0}^{j-1} \beta_{j-2,q} \left(x_0 + \Delta t \sum_{i=1}^q a_{q+1,i} k_i \right) \\ &= x_0 \sum_{q=0}^{j-1} \beta_{j-2,q} + \Delta t \sum_{q=0}^{j-1} \sum_{i=1}^q a_{q+1,i} k_i \\ &= x_0 \sum_{q=0}^{j-1} \beta_{j-2,q} + \Delta t \sum_{i=1}^{j-1} \sum_{q=i}^{j-1} a_{q+1,i} k_i. \end{aligned}$$

Now we impose the relation (4.4) for $k = j$, and we obtain

$$(4.5) \quad x_0 + \Delta t \left(\sum_{i=1}^j a_{1+j,i} k_i \right) \stackrel{!}{=} x_0 \sum_{q=0}^{j-1} \beta_{j-2,q} + \Delta t \sum_{i=1}^{j-1} \sum_{q=i}^{j-1} a_{q+1,i} k_i + \alpha_j \Delta t F(y_{j-1})$$

We have that, equating the coefficients of the k -terms, a sufficient condition for (4.5) to hold is

$$(4.6) \quad \begin{cases} \sum_{q=0}^{j-1} \beta_{j-2,q} = 1, \\ \sum_{q=i}^{j-1} \beta_{j-2,q} a_{q+1,i} = a_{j+1,i}, \\ \alpha_j = a_{j+1,j}. \end{cases} \quad \text{for } i = 1, \dots, j-1$$

This is a linear system of $j+1$ equations in $j+1$ unknowns. The system can be rewritten as $Ax = b$, where $\det A = \prod_{k=1}^j a_{k,k+1}$. We see that there exists a unique solution to the system in the conditions of the Proposition.

The induction step is therefore proved, and this proves the Proposition. \square

Remark 4.3. We remark that, solving system (4.6) successively for $j = 1, \dots, s$, one can obtain explicitly the form of the coefficients α and β .

In particular, we have the following Proposition.

Proposition 4.4. *A 3-stage Runge-Kutta method to solve the problem $y' = F(y)$ is a particular case of combination of 3 generalized midpoint steps.*

Proof. We begin by setting the equations: $F(y_j) = k_{j+1}$, for $j = 1, \dots, s$, and derive some conditions on the coefficients.

$$\begin{aligned} F(y_0) = k_1 &\implies y_0 = x_0, \\ F(y_1) = k_2 &\implies y_0 + \alpha_1 \Delta t F(y_0) = x_0 + \Delta t (a_{21} F(y_0)) \implies \alpha_1 = a_{21}, \\ F(y_2) = k_3 &\implies \beta_{00} y_0 + \beta_{01} y_1 + \alpha_2 \Delta t F(y_1) = x_0 + \Delta t (a_{31} k_1 + a_{32} k_2) \\ &\implies a_{32} = \alpha_2, \beta_{00} + \beta_{01} = 1, \alpha_1 \beta_{01} = a_{31}. \end{aligned}$$

We then solve:

$$(4.7) \quad \alpha_1 = a_{21}, \quad \beta_{01} = a_{31}/(a_{21}), \quad \beta_{00} = 1 - a_{31}/(a_{21}), \quad \alpha_2 = a_{32}.$$

Finally, we require $y_3 = x_3$, and we have

$$\begin{aligned} & \beta_{10}y_0 + \beta_{11}y_1 + \beta_{12}y_2 + \alpha_2\Delta tF(y_2) \\ &= \beta_{10}y_0 + \beta_{11}(y_0 + \alpha_1\Delta tF(y_0)) + \beta_{12}(\beta_{00}y_0 + \beta_{01}(y_0 + \alpha_1\Delta tF(y_0)) + \alpha_2\Delta tF(y_2)) + \alpha_3\Delta tF(y_2) \\ &= x_0 + b_1F(y_0) + b_2F(y_1) + b_3F(y_2). \end{aligned}$$

Hence it suffices that

$$(4.8) \quad \begin{aligned} \beta_{10} + \beta_{11} + \beta_{12} &= 1, \\ \beta_{11}\alpha_1 + \beta_{12}\beta_{01}\alpha_1 &= b_1, \\ \beta_{12}\alpha_2 &= b_2 \\ \alpha_3 &= b_3. \end{aligned}$$

So, if the coefficients $a_{i+1,i}$ are all nonzero, these equations can all be satisfied simultaneously. \square

Remark 4.5. We remark that the relations (4.7) and (4.8) are exactly the relations obtained in the general case, i.e. (4.6).

5. REMARKS ON 4TH ORDER SSPX

A 4th order SSPx takes the form

$$(5.1) \quad u_1 = u_0 + a_1\Delta tF(u_0),$$

$$(5.2) \quad \bar{u}_1 = (1 - w_1)u_0 + w_1u_1,$$

$$(5.3) \quad u_2 = \bar{u}_1 + a_2\Delta tF(u_1),$$

$$(5.4) \quad \bar{u}_2 = (1 - w_2 - w_3)u_0 + w_2u_1 + w_3u_2,$$

$$(5.5) \quad u_3 = \bar{u}_2 + a_3\Delta tF(u_2),$$

$$(5.6) \quad \bar{u}_3 = (1 - w_4 - w_5 - w_6)u_0 + w_4u_1 + w_5u_2 + w_6u_3,$$

$$(5.7) \quad u_4 = \bar{u}_3 + a_4\Delta tF(u_3).$$

The conditions for reaching 4th order are the following:

$$(5.8) \quad a_1a_2a_3a_4 = \frac{1}{24},$$

$$(5.9) \quad \begin{aligned} & \frac{1}{2}a_4(a_3(a_2 + a_1w_1)^2 + a_1^2a_2w_3 + 2(a_1a_3w_1 + a_2(a_3 + a_1w_3))(a_3 + a_2w_3 + a_1(w_2 + w_1w_3))) \\ & + \frac{1}{2}a_1a_2a_3(a_1 + 2a_2 + 2a_1w_1)w_6 = \frac{1}{6}, \end{aligned}$$

$$(5.10) \quad \frac{1}{6}(a_4(a_3 + a_2w_3 + a_1(w_2 + w_1w_3))^3 + a_1^3a_2w_5 + (a_3(a_2 + a_1w_1)^3 + a_1^3a_2w_3)w_6) = \frac{1}{24},$$

$$(5.11) \quad \frac{1}{2}(a_4(a_3 + a_2w_3 + a_1(w_2 + w_1w_3))^2 + a_1^2a_2w_5 + (a_3(a_2 + a_1w_1)^2 + a_1^2a_2w_3)w_6) = \frac{1}{6},$$

$$(5.12) \quad a_1a_3a_4w_1 + a_2(a_1a_4w_3 + a_3(a_4 + a_1w_6)) = \frac{1}{6},$$

$$(5.13) \quad a_2a_4w_3 + a_3(a_4 + (a_2 + a_1w_1)w_6) + a_1(a_4w_2 + a_4w_1w_3 + a_2w_5 + a_2w_3w_6) = \frac{1}{2},$$

$$(5.14) \quad a_4 + a_2w_5 + a_3w_6 + a_2w_3w_6 + a_1(w_4 + w_1w_5 + w_2w_6 + w_1w_3w_6) = 1.$$

We can reduce the system in the following way.

- (1) From Equation (5.12), we obtain w_6 in terms of w_1 and w_3 (such equation is linear in w_6):
 $w_6 = F_1(w_1, w_3).$

- (2) From Equation (5.9), we obtain w_2 in terms of w_1 and w_3 (and w_6 , but we substitute from point (1)): $w_2 = F_2(w_1, w_3)$.
- (3) From Equation (5.13), we obtain w_5 in terms of w_2, w_3, w_1, w_6 . Upon substitution, $w_5 = F_3(w_1, w_3)$.
- (4) From Equation (5.14), we obtain w_4 in terms of w_1, w_2, w_3, w_5, w_6 . Upon substitution, $w_4 = F_4(w_1, w_3)$.
- (5) We finally substitute into Equations (5.10) and (5.11). We obtain a nonlinear system of two equations in two unknowns.

Unlike the 3rd order method, there does not seem to be a solution when $a_1 = a_2 = a_3 = a_4 = 24^{-\frac{1}{4}}$.

Recall that the optimal a_{\max} we obtained from the 3rd order 3-step method was $(1/6)^{1/3} \sim 0.55$. The best a_{\max} I could obtain (by a very rough heuristic search) now is 9/10. The corresponding values of a_1, a_2, a_3, a_4 are the following:

$$a_1 = 9/10, a_2 = 4/5, a_3 = 1/10, a_4 = 125/216.$$

For these values, there is a 4th order 4 steps SSPx algorithm. The improvement on timestep is quite small, and I need to optimize this result. All these calculations are in the Mathematica file.